\begin{enumerate}
	\item Consider the following expressions
	\[p \implies (q \lor r), (p \land (\shortsim q)) \implies r, (p \land (\shortsim r)) \implies q.\]
	Show that the above expressions are logically equivalent\ldots
	\begin{itemize}
		\item directly by using a truth table.
		\item simplifying expressions using the rules in the table.
	\end{itemize}
	
	\item Simplify the expression
	\[z \land ((q \lor ((\shortsim w) \land q )) \land (( \shortsim z) \lor (\shortsim q)))\]
	as much as possible.
\end{enumerate}